Auto/Translation/LCtx.lean
@@ -1,0 +1,48 @@
+@[reducible] def pushLCtx (lctx : Nat → α) (x : α) : Nat → α
+| 0     => x
+| n + 1 => lctx n
+
+@[reducible] def pushLCtxDep {f : Nat → Sort u} (lctx : ∀ n, f n) (x : α) : ∀ n, (pushLCtx f α n)
+| 0     => x
+| n + 1 => lctx n
+
+def pushLCtxAt (lctx : Nat → α) (x : α) : (pos : Nat) → Nat → α
+| 0 => pushLCtx lctx x
+| pos' + 1 => fun n =>
+  match n with
+  | 0 => lctx 0
+  | n' + 1 => pushLCtxAt (fun n => lctx (Nat.succ n)) x pos' n'
+
+def pushLCtxAt_eqpos_cast₁ (lctx : Nat → α) (x : α) (pos : Nat) (f : α → Sort v)
+  (H : f (pushLCtxAt lctx x pos pos)) : f x :=
+  match pos with
+  | 0 => H
+  | pos' + 1 => pushLCtxAt_eqpos_cast₁ _ x pos' f H
+
+def pushLCtxAt_eqpos_cast₂ (lctx : Nat → α) (x : α) (pos : Nat) (f : α → Sort v)
+  (H : f x) : f (pushLCtxAt lctx x pos pos) :=
+  match pos with
+  | 0 => H
+  | pos' + 1 => pushLCtxAt_eqpos_cast₂ _ x pos' f H
+
+def popLCtx (lctx : Nat → α) := fun n => lctx (n + 1)
+
+def popLCtxs (lctx : Nat → α) (i : Nat) := fun n => lctx (Nat.add n i)
+
+-- Definitional equality :
+--   popLCtx (pushLCtx lctx x) = lctx x
+-- #reduce fun lctx x => popLCtx (pushLCtx lctx x)
+--   popLCtxs lctx 0 = lctx
+-- #reduce fun lctx => popLCtxs lctx 0
+-- #reduce fun lctx x => pushLCtxAt lctx x (pos:=2) 4
+-- #reduce (fun lctx x y t => (Eq.refl _ :
+--   pushLCtx (pushLCtxAt lctx x t) y = pushLCtxAt (pushLCtx lctx y) x (t + 1)))
+
+def push_pop_eq (lctx : Nat → α) :
+  pushLCtx (popLCtx lctx) (lctx 0) = lctx := by
+  apply funext
+  intro n; cases n <;> rfl
+
+theorem pushLCtx.comm (f : α → β) (lctx : Nat → α) (x : α) :
+  (fun n => f (pushLCtx lctx x n)) = pushLCtx (fun n => f (lctx n)) (f x) := by
+  apply funext; intro n; cases n <;> simp
